---
date: 2023-10-14
tags:
  - quantum-theory
---
$\hat{f}\psi = \lambda \psi \implies \mathbb{E}[f^m] = \braket{(\hat{f})^m}_\psi =\lambda^m$

>[!info]-
> 1. $\psi \in H$ is a [[quantum state vector]]
> 2. $f$ is a [[ðŸ“˜ Classical observable]]
> 3. $\hat{f}$ is the corresponding [[ðŸ“˜ Quantum observable]]
> 4. $\lambda \in \mathbb{R}, m \in \mathbb{Z}^+$ 

>[!success]
> $\mathbb{E}[f^m] = \braket{\psi, ( \hat{f} )^m \psi} = \braket{\psi, \lambda^m \psi} = \lambda^m \braket{\psi, \psi} = \lambda^m \| \psi \| = \lambda^m$.
> 
> The first equality holds since [[ðŸ“• The expectation of a physical observable is described by its self adjoint operator]] 
